DS/TernarySearchTree.v
@@ -1,6 +1,0 @@
-(** Ternary Search Tree (a data structure for storing finite collections
-    of strings:
-
-    https://www.drdobbs.com/database/ternary-search-trees/184410528
-
-*)
